Make thread_local a bit more consistent.
Make names more consistent with the rest of the development, make
definitions type classes opaque so that the proofmode does not unfold
then, declare timeless, persistent and proper instances.

program_logic/thread_local.v
@@ -2,44 +2,52 @@ From iris.algebra Require Export gmap gset coPset.
 From iris.proofmode Require Import invariants tactics.
 Import uPred.
 
+Definition tlN : namespace := nroot .@ "tl".
 Definition thread_id := gname.
 
 Class thread_localG Σ :=
   tl_inG :> inG Σ (prodR coPset_disjR (gset_disjR positive)).
 
-Definition tlN : namespace := nroot .@ "tl".
-
 Section defs.
   Context `{irisG Λ Σ, thread_localG Σ}.
 
-  Definition tl_tokens (tid : thread_id) (E : coPset) : iProp Σ :=
+  Definition tl_own (tid : thread_id) (E : coPset) : iProp Σ :=
     own tid (CoPset E, ∅).
 
   Definition tl_inv (tid : thread_id) (N : namespace) (P : iProp Σ) : iProp Σ :=
     (∃ i, ■ (i ∈ nclose N) ∧
-          inv tlN (P ★ own tid (∅, GSet {[i]}) ∨ tl_tokens tid {[i]}))%I.
+          inv tlN (P ★ own tid (∅, GSet {[i]}) ∨ tl_own tid {[i]}))%I.
 End defs.
 
-Instance: Params (@tl_tokens) 2.
 Instance: Params (@tl_inv) 4.
+Typeclasses Opaque tl_own tl_inv.
 
 Section proofs.
   Context `{irisG Λ Σ, thread_localG Σ}.
 
-  Lemma tid_alloc : True =r=> ∃ tid, tl_tokens tid ⊤.
+  Global Instance tl_own_timeless tid E : TimelessP (tl_own tid E).
+  Proof. rewrite /tl_own; apply _. Qed.
+
+  Global Instance tl_inv_ne tid N n : Proper (dist n ==> dist n) (tl_inv tid N).
+  Proof. rewrite /tl_inv. solve_proper. Qed.
+  Global Instance tl_inv_proper tid N : Proper ((≡) ==> (≡)) (tl_inv tid N).
+  Proof. apply (ne_proper _). Qed.
+
+  Global Instance tl_inv_persistent tid N P : PersistentP (tl_inv tid N P).
+  Proof. rewrite /tl_inv; apply _. Qed.
+
+  Lemma tl_alloc : True =r=> ∃ tid, tl_own tid ⊤.
   Proof. by apply own_alloc. Qed.
 
-  Lemma tl_tokens_disj tid E1 E2 :
-    tl_tokens tid E1 ★ tl_tokens tid E2 ⊢ ■ (E1 ⊥ E2).
+  Lemma tl_own_disjoint tid E1 E2 : tl_own tid E1 ★ tl_own tid E2 ⊢ ■ (E1 ⊥ E2).
   Proof.
-    rewrite /tl_tokens -own_op own_valid -coPset_disj_valid_op discrete_valid.
-    by iIntros ([? _]).
+    rewrite /tl_own -own_op own_valid -coPset_disj_valid_op. by iIntros ([? _]).
   Qed.
 
-  Lemma tl_tokens_union tid E1 E2 :
-    E1 ⊥ E2 → tl_tokens tid (E1 ∪ E2) ⊣⊢ tl_tokens tid E1 ★ tl_tokens tid E2.
+  Lemma tl_own_union tid E1 E2 :
+    E1 ⊥ E2 → tl_own tid (E1 ∪ E2) ⊣⊢ tl_own tid E1 ★ tl_own tid E2.
   Proof.
-    intros ?. by rewrite /tl_tokens -own_op pair_op left_id coPset_disj_union.
+    intros ?. by rewrite /tl_own -own_op pair_op left_id coPset_disj_union.
   Qed.
 
   Lemma tl_inv_alloc tid E N P : ▷ P ={E}=> tl_inv tid N P.
@@ -55,19 +63,20 @@ Section proofs.
       eapply nclose_infinite, (difference_finite_inv _ _), Hfin.
       apply of_gset_finite. }
     simpl. iDestruct "Hm" as %(<- & i & -> & ?).
-    iVs (inv_alloc tlN with "[-]"). 2:iVsIntro; iExists i; eauto.
+    rewrite /tl_inv.
+    iVs (inv_alloc tlN with "[-]"); last (iVsIntro; iExists i; eauto).
     iNext. iLeft. by iFrame.
   Qed.
 
   Lemma tl_inv_open tid tlE E N P :
     nclose tlN ⊆ tlE → nclose N ⊆ E →
-    tl_inv tid N P ⊢ tl_tokens tid E ={tlE}=★ ▷ P ★ tl_tokens tid (E ∖ N) ★
-                       (▷ P ★ tl_tokens tid (E ∖ N) ={tlE}=★ tl_tokens tid E).
+    tl_inv tid N P ⊢ tl_own tid E ={tlE}=★ ▷ P ★ tl_own tid (E ∖ N) ★
+                       (▷ P ★ tl_own tid (E ∖ N) ={tlE}=★ tl_own tid E).
   Proof.
-    iIntros (??) "#Htlinv Htoks".
-    iDestruct "Htlinv" as (i) "[% #Hinv]".
+    rewrite /tl_inv. iIntros (??) "#Htlinv Htoks".
+    iDestruct "Htlinv" as (i) "[% Hinv]".
     rewrite {1 4}(union_difference_L (nclose N) E) //.
-    rewrite {1 5}(union_difference_L {[i]} (nclose N)) ?tl_tokens_union; try set_solver.
+    rewrite {1 5}(union_difference_L {[i]} (nclose N)) ?tl_own_union; [|set_solver..].
     iDestruct "Htoks" as "[[Htoki $] $]".
     iInv tlN as "[[$ >Hdis]|>Htoki2]" "Hclose".
     - iVs ("Hclose" with "[Htoki]") as "_"; first auto.
@@ -77,7 +86,7 @@ Section proofs.
         iDestruct (own_valid with "Hdis") as %[_ Hval].
         revert Hval. rewrite gset_disj_valid_op. set_solver.
       + iFrame. iApply "Hclose". iNext. iLeft. by iFrame.
-    - iDestruct (tl_tokens_disj tid {[i]} {[i]} with "[-]") as %?. by iFrame.
+    - iDestruct (tl_own_disjoint tid {[i]} {[i]} with "[-]") as %?; first by iFrame.
       set_solver.
   Qed.
 End proofs.
